better sim relation, fix broken lemmas

LambdaDollarToLet.v
@@ -2,59 +2,55 @@ Require Export Common.
 Require Export LambdaDollar.
 Require Export LambdaLetDollar.
 
+Inductive sim_J_F {A} (R : tm A → tm' A → Prop) : J A → J' A → Prop :=
+| sim_J_fun : ∀ (e : tm  A) (e' : tm'  A), R e e' → sim_J_F R (J_fun e) (J_fun' e')
+| sim_J_arg : ∀ (v : val A) (v' : val' A), R v v' → sim_J_F R (J_arg v) (J_arg' v')
+| sim_J_dol : ∀ (e : tm  A) (e' : tm'  A), R e e' → sim_J_F R (J_dol e) (J_dol' e')
+.
 Reserved Notation "e ~ₑ e'" (at level 40).
 Reserved Notation "v ~ᵥ v'" (at level 40).
 Reserved Notation "p ~ₚ p'" (at level 40).
 Reserved Notation "j ~ⱼ j'" (at level 40).
 Reserved Notation "k ~ₖ k'" (at level 40).
 Reserved Notation "t ~ₜ t'" (at level 40).
-Inductive sim_J {A} : J A → J' A → Prop :=
-| sim_J_fun : ∀ e e', e ~ₑ e' → J_fun e ~ⱼ J_fun' e'
-| sim_J_arg : ∀ v v', v ~ᵥ v' → J_arg v ~ⱼ J_arg' v'
-| sim_J_dol : ∀ e e', e ~ₑ e' → J_dol e ~ⱼ J_dol' e'
-with sim_T {A} : T A → T' A → Prop :=
-| sim_T_nil  : T_nil ~ₜ T_nil'
-| sim_T_cons : ∀ v v' k k' t t', T_cons v k t ~ₜ T_cons' v' k' t'
-with sim_K {A} : K A → K' A → Prop :=
-| sim_K_nil  : K_nil ~ₖ K_nil'
-| sim_K_cons : ∀ j j' k k',
-    j ~ⱼ j' → k ~ₖ k' →
-    K_cons j k ~ₖ K_let' k' <| ↑j'[0] |> (* J[K] ~ let x = K' in J'[0] *)
-with sim_val {A} : val A → val' A → Prop :=
-| sim_val_abs : ∀ e e', tm_abs e ~ₑ tm_abs' e' → val_abs e ~ᵥ val_abs' e'
-with sim_non {A} : non A → non' A → Prop :=
-| sim_non_ : ∀ p p', non_to_tm p ~ₑ non_to_tm' p' → p ~ₚ p'
-with sim_tm {A} : tm A → tm' A → Prop :=
+Inductive sim_tm {A} : tm A → tm' A → Prop :=
 | sim_var  : ∀ a, <{ var a }> ~ₑ <| var a |>
 | sim_abs  : ∀ e e', e ~ₑ e' → <{ λ  e }> ~ₑ <| λ  e' |>
 | sim_s_0  : ∀ e e', e ~ₑ e' → <{ S₀ e }> ~ₑ <| S₀ e' |>
 | sim_app  : ∀ e1 e2 e1' e2', e1 ~ₑ e1' → e2 ~ₑ e2' → <{ e1   e2 }> ~ₑ <| e1'   e2' |>
 | sim_dol  : ∀ e1 e2 e1' e2', e1 ~ₑ e1' → e2 ~ₑ e2' → <{ e1 $ e2 }> ~ₑ <| e1' $ e2' |>
-(* | sim_plug : ∀ k k' e e', k ~ₖ k' → e ~ₑ e' → plugK k e ~ₑ plugK' k' e' *)
-| sim_cont : ∀ v v' k k' e e',
-    v ~ᵥ v' → k ~ₖ k' → e ~ₑ e' →
-    <{ λ {liftV  v } $ ↑k [0] }> ~ₑ <| λ {liftV' v'} $ ↑k'[0] |>
+| sim_let  : ∀ j j' e e', j ~ⱼ j' → e ~ₑ e' → <{ j [e] }> ~ₑ <| let e' in ↑j'[0] |>
 where "e ~ₑ e'" := (sim_tm  e e')
-and   "v ~ᵥ v'" := (sim_val v v')
-and   "p ~ₚ p'" := (sim_non p p')
-and   "j ~ⱼ j'" := (sim_J   j j')
-and   "k ~ₖ k'" := (sim_K   k k')
-and   "t ~ₜ t'" := (sim_T   t t').
-Global Hint Constructors sim_J : core.
+and   "j ~ⱼ j'" := (sim_J_F sim_tm j j').
+Inductive sim_val {A} : val A → val' A → Prop :=
+| sim_val_abs : ∀ e e', tm_abs e ~ₑ tm_abs' e' → val_abs e ~ᵥ val_abs' e'
+where "v ~ᵥ v'" := (sim_val v v').
+Inductive sim_non {A} : non A → non' A → Prop :=
+| sim_non_ : ∀ p p', non_to_tm p ~ₑ non_to_tm' p' → p ~ₚ p'
+where "p ~ₚ p'" := (sim_non p p').
+Inductive sim_K {A} : K A → K' A → Prop :=
+| sim_K_nil  :
+    K_nil ~ₖ K_nil'
+| sim_K_cons : ∀ j j' k k',
+    j ~ⱼ j' →
+    k ~ₖ k' →
+    K_cons j k ~ₖ K_let' k' <| ↑j'[0] |> (* J[K] ~ let x = K' in J'[0] *)
+where "k ~ₖ k'" := (sim_K k k').
+Inductive sim_T {A} : T A → T' A → Prop :=
+| sim_T_nil  :
+    T_nil ~ₜ T_nil'
+| sim_T_cons : ∀ v v' k k' t t',
+    v ~ᵥ v' →
+    k ~ₖ k' →
+    t ~ₜ t' →
+    T_cons v k t ~ₜ T_cons' v' k' t'
+where "t ~ₜ t'" := (sim_T t t').
+Global Hint Constructors sim_J_F : core.
 Global Hint Constructors sim_K : core.
 Global Hint Constructors sim_T : core.
 Global Hint Constructors sim_val : core.
 Global Hint Constructors sim_non : core.
 Global Hint Constructors sim_tm : core.
-
-Reserved Notation "e ~ e'" (at level 40).
-Inductive sim_toplevel {A} : tm A → tm' A → Prop :=
-| sim_top_base : ∀ e e', e ~ₑ e' → e ~ e'
-| sim_top_cons : ∀ k k' t t' e e',
-    k ~ₖ k' → t ~ₜ t' → e ~ₑ e' → 
-    <{ k[t[e]] }> ~ <| k'[t'[e']] |>
-where "e ~ e'" := (sim_toplevel e e').
-Global Hint Constructors sim_toplevel : core.
 
 Lemma sim_tm_from_sim_val : ∀ {A v} {v' : val' A},
   v ~ᵥ v' →
@@ -62,15 +58,14 @@ Lemma sim_tm_from_sim_val : ∀ {A v} {v' : val' A},
 Proof.
   intros. destruct v, v'. inversion H; clear H; subst. assumption.
 Qed.
+Global Hint Resolve sim_tm_from_sim_val : core.
 
 Lemma sim_val_inv : ∀ {A} (v : val A) (e' : tm' A),
   v ~ₑ e' → ∃ (v' : val' A), e' = v' /\ v ~ᵥ v'.
 Proof.
   intros. destruct v. inversion H; clear H; subst.
   exists (val_abs' e'0); auto.
-  exists (val_abs' <| {liftV' v'} $ ↑k'[0] |>); split; auto.
-  constructor.
-  eapply (sim_cont v v' k k'); eassumption.
+  destruct j; inversion H0.
 Qed.
 
 Lemma sim_non_inv : ∀ {A} (p : non A) (e' : tm' A),
@@ -78,20 +73,44 @@ Lemma sim_non_inv : ∀ {A} (p : non A) (e' : tm' A),
 Proof.
   intros. destruct p; inversion H; clear H; subst.
   exists (non_s_0' e'0); split; auto; repeat constructor; assumption.
+  destruct j; inversion H0.
   exists (non_app' e1' e2'); split; auto; repeat constructor; assumption.
+  exists (non_let' e'0 <| ↑j'[0] |>); split; auto; constructor; cbn; rewrite <- H0; auto.
   exists (non_dol' e1' e2'); split; auto; repeat constructor; assumption.
+  exists (non_let' e'0 <| ↑j'[0] |>); split; auto; constructor; cbn; rewrite <- H0; auto.
 Qed.
 
-Lemma sim_j_inv : ∀ (j : J ␀) e term',
-  <{ j[e] }> ~ₑ term' → ∃ j' e', j ~ⱼ j' /\ e ~ₑ e' /\ term' = <| j'[e'] |>.
+Ltac reason := repeat(
+  match goal with
+  | H : val_to_tm ?v ~ₑ ?e' |- _ =>
+      let v' := fresh "v'" in
+      let Hev := fresh "Hev" in
+      let Hv := fresh "Hv" in
+      apply sim_val_inv in H as [v' [Hev Hv]]; subst
+  | H : val_to_tm' ?v1 = val_to_tm' ?v2 |- _ => apply val_to_tm_injection' in H
+  | H : val_to_tm  ?v1 = val_to_tm  ?v2 |- _ => apply val_to_tm_injection  in H
+  end).
+
+(* Lemma sim_j_inv : ∀ (j : J ␀) e term',
+  <{ j[e] }> ~ₑ term' →
+  ∃ j' e', j ~ⱼ j' /\ e ~ₑ e' /\ (term' = <| j'[e'] |> \/ term' = <| let e' in ↑j'[0] |>).
 Proof.
-  intros. inversion H; clear H; subst;
-    try destruct a; 
-    destruct j; inversion H0; clear H0; subst; cbn in *;
-    try solve [repeat eexists; eauto].
-  apply sim_val_inv in H1 as [v' [Hvv Hv]]; subst.
+  intros. inversion H; clear H; subst.
+  admit. admit. admit. admit. admit.
+  destruct j0, j; cbn in H0; inversion H0; clear H0; subst.
   repeat eexists; eauto.
-Qed.
+  apply sim_val_inv in H2 as [v' [Hev Hv]]; subst. exists (J_arg' v'); inversion H1; clear H1; subst. repeat eexists; eauto. constructor.
+  repeat eexists; eauto.
+  inversion H0.
+  try destruct a;
+    try destruct a; 
+  try destruct a;
+  destruct j; inversion H0; clear H0; subst; cbn in *;
+  try solve [repeat eexists; eauto].
+  apply sim_val_inv in H1 as [v' [Hvv Hv]]; subst.
+  repeat eexists. constructor. apply (sim_tm_from_sim_val Hv). apply H2. auto.
+  repeat eexists. constructor.
+Qed. *)
 
 (* k[p] ~ e' -->'* k'[p'] *)
 Lemma plug_k_steps_to_similar_k' : ∀ (k : K ␀) (p : non ␀) term',
@@ -104,15 +123,65 @@ Proof.
   induction k; intros; cbn in *.
   - apply sim_non_inv in H as [p' [H Hp]]; subst.
     exists K_nil'; exists p'; auto.
-  - apply sim_j_inv in H as [j' [e' [Hj [Hke Hje]]]]; subst.
-    apply IHk in Hke as [k' [p'' [Hstep [Hk He]]]].
+  - inversion H; clear H; subst;
+    try solve [destruct j; inversion H1 + inversion H0].
+
+    destruct j; inversion H0; clear H0; subst. 
+    apply IHk in H1 as [k' [p'' [Hstep [Hk He]]]].
     inversion He; clear He; subst. 
+    repeat eexists; eauto. cbn.
     apply (non_when_steps_to_plug_non' _ _ T_nil') in Hstep as Haux. destruct Haux as [p' HH]. subst.
-    exists (K_let' k' <| ↑j'[0] |>). exists p''. cbn.
-    repeat split; auto.
-    apply (multi_contr_multi' (contr_let' j' p')).
-    apply (multi_let'). apply Hstep.
-  Qed.
+    apply (multi_contr_multi' (contr_let' (J_fun' e2') p')); cbn.
+    apply (multi_let' Hstep).
+
+    apply sim_val_inv in H1 as [v' [Hev Hv]]; subst.
+    apply IHk in H2 as [k' [p'' [Hstep [Hk He]]]].
+    inversion He; clear He; subst. 
+    repeat eexists; eauto; cbn.
+    apply (non_when_steps_to_plug_non' _ _ T_nil') in Hstep as Haux. destruct Haux as [p' HH]. subst.
+    apply (multi_contr_multi' (contr_let' (J_arg' v') p')); cbn.
+    apply (multi_let' Hstep).
+
+    destruct j; inversion H0; clear H0; subst. 
+    apply IHk in H1 as [k' [p'' [Hstep [Hk He]]]].
+    inversion He; clear He; subst. 
+    repeat eexists; eauto. cbn.
+    apply (non_when_steps_to_plug_non' _ _ T_nil') in Hstep as Haux. destruct Haux as [p' HH]. subst.
+    apply (multi_contr_multi' (contr_let' (J_dol' e2') p')); cbn.
+    apply (multi_let' Hstep).
+
+    destruct j0, j; inversion H0; clear H0; subst; inversion H1; clear H1; subst; reason.
+
+    apply IHk in H2 as [k' [p'' [Hstep [Hk He]]]];
+    inversion He; clear He; subst;
+    apply (non_when_steps_to_plug_non' _ _ T_nil') in Hstep as Haux; destruct Haux as [p' HH]; subst;
+    exists (K_let' k' <| 0 ↑e'0 |>); exists p''; cbn; repeat split; auto;
+    [ apply (multi_let' Hstep) | apply (sim_K_cons _ (J_fun' e'0)); auto ].
+
+    apply IHk in H0 as [k' [p'' [Hstep [Hk He]]]];
+    inversion He; clear He; subst;
+    apply (non_when_steps_to_plug_non' _ _ T_nil') in Hstep as Haux; destruct Haux as [p' HH]; subst; cbn.
+    eexists (K_let' k' _); repeat eexists; cbn.
+    apply (multi_contr_multi' (contr_let_beta' _ _)).
+    change (tm_subst0' <| 0 {↑ (non_to_tm' p')} |> v') with <| v' {tm_subst0' (↑(non_to_tm' p')) v'} |>.
+    rewrite subst_lift'.
+    apply (multi_contr_multi' (contr_let' (J_arg' v') _)); cbn.
+    apply (multi_let' Hstep). apply (sim_K_cons _ (J_arg' v')); auto. auto.
+
+    destruct k; cbn in *; inversion H3; destruct v; [destruct p | destruct j]; inversion H0.
+
+    apply IHk in H2 as [k' [p'' [Hstep [Hk He]]]];
+    inversion He; clear He; subst;
+    apply (non_when_steps_to_plug_non' _ _ T_nil') in Hstep as Haux; destruct Haux as [p' HH]; subst;
+    exists (K_let' k' <| {liftV' v'0} 0 |>); exists p''; cbn; repeat split; auto;
+    [ apply (multi_let' Hstep) | apply (sim_K_cons _ (J_arg' v'0)); auto ].
+
+    apply IHk in H2 as [k' [p'' [Hstep [Hk He]]]];
+    inversion He; clear He; subst;
+    apply (non_when_steps_to_plug_non' _ _ T_nil') in Hstep as Haux; destruct Haux as [p' HH]; subst.
+    exists (K_let' k' <| 0 $ ↑e'0 |>); exists p''; cbn; repeat split; auto;
+    [ apply (multi_let' Hstep) | apply (sim_K_cons _ (J_dol' e'0)); auto ].
+Qed.
 
 Lemma plug_t_steps_to_similar_t' : ∀ (t : T ␀) (p : non ␀) term',
   <{ t [p] }> ~ₑ term' →
@@ -136,7 +205,23 @@ Proof.
     apply multi_delim'.
     apply (multi_trans Hmulti1).
     apply multi_k'. apply Hmulti2.
-  Qed.
+
+    destruct j; cbn in H0; inversion H0; clear H0; subst.
+    reason.
+    inversion H1; clear H1; subst.
+    destruct (plug_non_is_non K_nil t p) as [tp Htp]; cbn in Htp. rewrite Htp in H0.
+    apply plug_k_steps_to_similar_k' in H0 as [k' [p' [Hmulti1 [Hk Hp]]]].
+    inversion Hp; clear Hp; subst. rewrite <- Htp in *.
+    apply IHt in H as [t' [p'' [Hmulti2 [Ht Hp2]]]].
+    inversion Hp2; clear Hp2; subst. 
+    exists (T_cons' v' k' t'). repeat eexists; eauto. cbn.
+    apply (multi_contr_multi' (contr_let_beta' v' _)).
+    change (tm_subst0' <| 0 $ ↑ (e') |> v') with <| v' $ (↑e')[0 := v'] |>.
+    apply multi_delim'.
+    rewrite subst_lift'.
+    apply (multi_trans Hmulti1).
+    apply (multi_k' Hmulti2).
+Qed.
 
 Lemma plug_kt_steps_to_similar_kt' : ∀ (k : K ␀) (t : T ␀) (p : non ␀) term',
   <{ k [t [p]] }> ~ₑ term' →
